theories/Weakening.v
@@ -311,3 +311,4 @@ Ltac bsimpl := check_no_evars;
                   Up_term_term, Up_term, up_term, Subst_term, Subst1, subst1,
                   Ren1_subst, Ren1_wk, Ren1_well_wk, Ren_decl
                   in *; bsimpl'; minimize.
+
